case_study/RiscvPmp/Contracts.v
@@ -973,7 +973,7 @@ Section ContractDefKit.
     |}.
 
   Definition sep_contract_step {τ Δ} : SepContract Δ τ :=
-    let Σ := ["m" :: ty_privilege; "h" :: ty_xlenbits; "i" :: ty_xlenbits; "entries" :: ty_list ty_pmpentry; "mpp" :: ty_privilege; "mepc" :: ty_xlenbits; "npc" :: ty_xlenbits] in
+    let Σ := ["m" :: ty_privilege; "h" :: ty_xlenbits; "entries" :: ty_list ty_pmpentry; "mpp" :: ty_privilege; "mepc" :: ty_xlenbits; "i" :: ty_xlenbits; "npc" :: ty_xlenbits] in
     {| sep_contract_logic_variables := sep_contract_logvars Δ Σ;
        sep_contract_localstore      := create_localstore Δ Σ;
        sep_contract_precondition    :=
